step 3: split QUIC.Parse.* into Spec and Impl

src/QUIC.Impl.VarInt.fsti
@@ -1,31 +1,9 @@
-module QUIC.Parse.VarInt
-include QUIC.Spec.Base
+module QUIC.Impl.VarInt
+include QUIC.Spec.VarInt
 
 module U64 = FStar.UInt64
 module LP = LowParse.Spec.BoundedInt // for bounded_int32
 module LL = LowParse.Low.Base
-
-inline_for_extraction
-let parse_varint_kind = {
-  LP.parser_kind_low = 1;
-  LP.parser_kind_high = Some 8;
-  LP.parser_kind_subkind = Some LP.ParserStrong;
-  LP.parser_kind_metadata = None;
-}
-
-val parse_varint : LP.parser parse_varint_kind uint62_t
-
-val serialize_varint : LP.serializer parse_varint
-
-val parse_bounded_varint
-  (min: nat)
-  (max: nat { min <= max /\ max < 4294967296 })
-: Tot (LP.parser parse_varint_kind (LP.bounded_int32 min max))
-
-val serialize_bounded_varint
-  (min: nat)
-  (max: nat { min <= max /\ max < 4294967296 })
-: Tot (LP.serializer (parse_bounded_varint min max))
 
 val validate_varint: LL.validator parse_varint
 
@@ -33,7 +11,7 @@ val read_varint: LL.leaf_reader parse_varint
 
 val jump_varint: LL.jumper parse_varint
 
-val serialize_varint_impl: LL.serializer32 serialize_varint
+val serialize_varint: LL.serializer32 serialize_varint
 
 module U32 = FStar.UInt32
 
@@ -58,8 +36,7 @@ val jump_bounded_varint
 
 inline_for_extraction
 noextract
-val serialize_bounded_varint_impl
+val serialize_bounded_varint
   (min: nat)
   (max: nat { min <= max /\ max < 4294967296 })
 : Tot (LL.serializer32 (serialize_bounded_varint min max))
-
