src/QUIC.Spec.Header.fst
@@ -1,8 +1,6 @@
-module QUIC.Parse
+module QUIC.Spec.Header
 open QUIC.Spec.Base
-open QUIC.Parse.PacketNumber
-
-open FStar.HyperStack.ST
+open QUIC.Spec.PacketNumber
 
 open LowParse.Spec.Int
 open LowParse.Spec.BitSum
@@ -15,6 +13,7 @@ module U16 = FStar.UInt16
 module U8 = FStar.UInt8
 
 (* From https://tools.ietf.org/html/draft-ietf-quic-transport-23#section-17 *)
+
 
 inline_for_extraction
 noextract
@@ -325,7 +324,7 @@ let header_synth
 let parse_common_long : parser _ common_long_t =
   parse_u32 `nondep_then` (parse_bounded_vlbytes 0 20 `nondep_then` parse_bounded_vlbytes 0 20)
 
-open QUIC.Parse.VarInt
+open QUIC.Spec.VarInt
 
 let parse_payload_length_pn
   (last: last_packet_number_t)
@@ -461,88 +460,11 @@ let serialize_header_eq
     (serialize_header_body short_dcid_len last)
     x
 
-module LC = LowParse.Low.Combinators
-module LB = LowParse.Low.Bytes
-module LI = LowParse.Low.BoundedInt
-module LJ = LowParse.Low.Int
-module LL = LowParse.Low.BitSum
-
-inline_for_extraction
-let validate_common_long : LC.validator parse_common_long =
-  LB.validate_u32 () `LC.validate_nondep_then` (LB.validate_bounded_vlbytes 0 20 `LC.validate_nondep_then` LB.validate_bounded_vlbytes 0 20)
-
-inline_for_extraction
-noextract
-let validate_payload_length_pn
-  (last: last_packet_number_t)
-  (pn_length: packet_number_length_t)
-: Tot (LC.validator (parse_payload_length_pn last pn_length))
-= validate_varint `LC.validate_nondep_then` validate_packet_number last pn_length
-
-[@filter_bitsum'_t_attr]
-inline_for_extraction
-noextract
-let validate_header_body_cases
-  (short_dcid_len: short_dcid_len_t)
-  (last: last_packet_number_t)
-  (k' : bitsum'_key_type first_byte)
-: Tot (LC.validator (dsnd (parse_header_body short_dcid_len last k')))
-= match coerce (bitsum'_key_type first_byte) k' with
-  | (| Short, (| (), (| (), (| pn_length, () |) |) |) |) ->
-    LC.validate_weaken (strong_parser_kind 0 20 None) (LB.validate_flbytes (U32.v short_dcid_len) short_dcid_len) () `LC.validate_nondep_then` validate_packet_number last pn_length
-  | (| Long, (| (), (| Initial, (| (), (| pn_length, () |) |) |) |) |) ->
-    validate_common_long `LC.validate_nondep_then` (LB.validate_bounded_vlgenbytes 0 0ul token_max_len (U32.uint_to_t token_max_len) (validate_bounded_varint 0ul (U32.uint_to_t token_max_len)) (read_bounded_varint 0 token_max_len) `LC.validate_nondep_then` validate_payload_length_pn last pn_length)
-  | (| Long, (| (), (| ZeroRTT, (| (), (| pn_length, () |) |) |) |) |) ->
-    validate_common_long `LC.validate_nondep_then` validate_payload_length_pn last pn_length
-  | (| Long, (| (), (| Handshake, (| (), (| pn_length, () |) |) |) |) |) ->
-    validate_common_long `LC.validate_nondep_then` validate_payload_length_pn last pn_length
-  | (| Long, (| (), (| Retry, () |) |) |) ->
-    validate_common_long `LC.validate_nondep_then` LB.validate_bounded_vlbytes 0 20
-
-let filter_first_byte'
-: (filter_bitsum'_t first_byte)
-= norm [primops; iota; zeta; delta_attr [`%filter_bitsum'_t_attr]]
-  (mk_filter_bitsum'_t' first_byte)
-
-inline_for_extraction
-let filter_first_byte
-  (short_dcid_len: short_dcid_len_t)
-  (last: last_packet_number_t)
-: Tot (filter_bitsum'_t first_byte)
-= coerce (filter_bitsum'_t first_byte) filter_first_byte'
-
-inline_for_extraction
-noextract
-let mk_validate_header_body_cases'
-: LL.validate_bitsum_cases_t first_byte
-= norm [primops; iota; zeta; delta_attr [`%filter_bitsum'_t_attr]]
-  (LL.mk_validate_bitsum_cases_t' first_byte)
-
-inline_for_extraction
-noextract
-let mk_validate_header_body_cases
-  (short_dcid_len: short_dcid_len_t)
-  (last: last_packet_number_t)
-: LL.validate_bitsum_cases_t first_byte
-= coerce (LL.validate_bitsum_cases_t first_byte) mk_validate_header_body_cases' 
-
-let validate_header
-  (short_dcid_len: short_dcid_len_t)
-  (last: last_packet_number_t)
-: Tot (LL.validator (lp_parse_header short_dcid_len last))
-= LL.validate_bitsum
-    first_byte
-    (first_byte_of_header short_dcid_len last)
-    (header_body_type short_dcid_len last)
-    (header_synth short_dcid_len last)
-    (LJ.validate_u8 ())
-    LJ.read_u8
-    (filter_first_byte short_dcid_len last)
-    (parse_header_body short_dcid_len last)
-    (validate_header_body_cases short_dcid_len last)
-    (mk_validate_header_body_cases short_dcid_len last)
-
-#pop-options
+module LC = LowParse.Spec.Combinators
+module LB = LowParse.Spec.Bytes
+module LI = LowParse.Spec.BoundedInt
+module LJ = LowParse.Spec.Int
+module LL = LowParse.Spec.BitSum
 
 (* Properties of the serializer *)
 
@@ -685,6 +607,8 @@ let lemma_header_parsing_correct
   | H_Failure -> ()
   | H_Success h' c' -> assert (h == h' /\ c `Seq.equal` c')
 
+#push-options "--z3rlimit 256"
+
 let lemma_header_parsing_safe
   cid_len last b1 b2
 = match parse_header cid_len last b1 with
@@ -703,335 +627,3 @@ let lemma_header_parsing_safe
     assert (parse_header cid_len last b2 == H_Success h1 c1);
     Seq.lemma_split b2 consumed;
     assert (b1 == b2)
-
-#pop-options
-
-module Impl = QUIC.Impl.Base
-
-inline_for_extraction
-noextract
-let destr_first_byte
-: (destr_bitsum'_t first_byte)
-= norm [primops; iota; zeta; delta_attr [`%filter_bitsum'_t_attr]]
-  (mk_destr_bitsum'_t first_byte)
-
-inline_for_extraction
-noextract
-let read_header_body_t
-  (sl: LL.slice (B.trivial_preorder _) (B.trivial_preorder _))
-  (cid_len: U32.t { U32.v cid_len < 20 } )
-  (last: uint62_t { U64.v last + 1 < pow2 62 })
-  (tg: bitsum'_type first_byte)
-: Tot (Type u#0)
-= (len: U32.t) ->
-  HST.Stack Impl.header
-  (requires (fun h ->
-    let p = dsnd (parse_header_body cid_len last (bitsum'_key_of_t first_byte tg)) in
-    LL.valid_pos (lp_parse_header cid_len last) h sl 0ul len /\
-    1 <= U32.v sl.LL.len /\
-    LL.valid_pos p h sl 1ul len /\
-    LL.contents (lp_parse_header cid_len last) h sl 0ul == (header_synth cid_len last).f tg (LL.contents p h sl 1ul)
-  ))
-  (ensures (fun h x h' ->
-    B.modifies B.loc_none h h' /\
-    begin
-      let hd = LL.contents (lp_parse_header cid_len last) h sl 0ul in
-      Impl.header_live x h' /\
-      LL.loc_slice_from_to sl 0ul len `B.loc_includes` Impl.header_footprint x /\
-      Impl.g_header x h' == hd
-    end
-  ))
-
-#push-options "--z3rlimit 64 --z3cliopt smt.arith.nl=false --using_facts_from '*,-FStar.Int.Cast' --query_stats --max_fuel 9 --initial_fuel 9 --max_ifuel 9 --initial_ifuel 9 --query_stats"
-
-let read_header_body_short
-  (sl: LL.slice (B.trivial_preorder _) (B.trivial_preorder _))
-  (cid_len: U32.t { U32.v cid_len < 20 } )
-  (last: uint62_t { U64.v last + 1 < pow2 62 })
-  (spin: BF.bitfield uint8 1)
-  (key_phase: BF.bitfield uint8 1)
-  (pn_length: packet_number_length_t)
-: Tot (read_header_body_t sl cid_len last (| Short, (| (), (spin, (| (), (key_phase, (| pn_length, () |) ) |) ) |) |) )
-= fun len ->
-    let h0 = HST.get () in
-    assert_norm (bitsum'_key_of_t first_byte (| Short, (| (), (spin, (| (), (key_phase, (| pn_length, () |) ) |) ) |) |) == (| Short, (| (), (| (), (| pn_length, () |) |) |) |) );
-    LL.valid_nondep_then h0 (weaken (strong_parser_kind 0 20 None) (parse_flbytes (U32.v cid_len))) (parse_packet_number last pn_length) sl 1ul;
-    LL.valid_weaken (strong_parser_kind 0 20 None) (parse_flbytes (U32.v cid_len)) h0 sl 1ul;
-    LB.valid_flbytes_elim h0 (U32.v cid_len) sl 1ul;
-    let pos = LB.jump_flbytes (U32.v cid_len) cid_len sl 1ul in
-    let dcid = B.sub sl.LL.base 1ul (pos `U32.sub` 1ul) in
-    let pn = read_packet_number last pn_length sl pos in
-    Impl.BShort (spin = 1uy) (key_phase = 1uy) dcid cid_len pn pn_length
-
-#pop-options
-
-#push-options "--z3rlimit 128 --z3cliopt smt.arith.nl=false --using_facts_from '*,-FStar.Int.Cast' --query_stats --max_fuel 9 --initial_fuel 9 --max_ifuel 9 --initial_ifuel 9 --query_stats"
-
-#restart-solver
-
-let read_header_body_long_retry
-  (sl: LL.slice (B.trivial_preorder _) (B.trivial_preorder _))
-  (cid_len: U32.t { U32.v cid_len < 20 } )
-  (last: uint62_t { U64.v last + 1 < pow2 62 })
-  (unused: BF.bitfield uint8 4)
-: Tot (read_header_body_t sl cid_len last (| Long, (| (), (| Retry, (unused, ()) |) |) |) )
-= fun len ->
-    let h0 = HST.get () in
-    assert_norm (bitsum'_key_of_t first_byte (| Long, (| (), (| Retry, (unused, ()) |) |) |)  == (| Long, (| (), (| Retry, () |) |) |) );
-    LL.valid_nondep_then h0 parse_common_long (parse_bounded_vlbytes 0 20) sl 1ul;
-    LL.valid_nondep_then h0 parse_u32 (parse_bounded_vlbytes 0 20 `nondep_then` parse_bounded_vlbytes 0 20) sl 1ul;
-    let version = LJ.read_u32 sl 1ul in
-    let pos1 = LJ.jump_u32 sl 1ul in
-    LL.valid_nondep_then h0 (parse_bounded_vlbytes 0 20) (parse_bounded_vlbytes 0 20) sl pos1;
-    let dcid = LB.get_vlbytes_contents 0 20 sl pos1 in
-    let dcid_len = LB.bounded_vlbytes_payload_length 0 20 sl pos1 in
-    let pos2 = LB.jump_bounded_vlbytes 0 20 sl pos1 in
-    let scid = LB.get_vlbytes_contents 0 20 sl pos2 in
-    let scid_len = LB.bounded_vlbytes_payload_length 0 20 sl pos2 in
-    let pos3 = LB.jump_bounded_vlbytes 0 20 sl pos2 in
-    let odcid = LB.get_vlbytes_contents 0 20 sl pos3 in
-    let odcid_len = LB.bounded_vlbytes_payload_length 0 20 sl pos3 in
-    let spec = Impl.BRetry unused odcid odcid_len in
-    Impl.BLong version dcid dcid_len scid scid_len spec
-
-#pop-options
-
-#push-options "--z3rlimit 512 --z3cliopt smt.arith.nl=false --using_facts_from '*,-FStar.Int.Cast' --query_stats --max_fuel 9 --initial_fuel 9 --max_ifuel 9 --initial_ifuel 9 --query_stats"
-
-#restart-solver
-
-let read_header_body_long_initial
-  (sl: LL.slice (B.trivial_preorder _) (B.trivial_preorder _))
-  (cid_len: U32.t { U32.v cid_len < 20 } )
-  (last: uint62_t { U64.v last + 1 < pow2 62 })
-  (pn_length: packet_number_length_t)
-: Tot (read_header_body_t sl cid_len last (| Long, (| (), (| Initial, (| (), (| pn_length, () |) |) |) |) |) )
-= fun len ->
-    let h0 = HST.get () in
-    assert_norm (bitsum'_key_of_t first_byte (| Long, (| (), (| Initial, (| (), (| pn_length, () |) |) |) |) |) == (| Long, (| (), (| Initial, (| (), (| pn_length, () |) |) |) |) |) );
-    LL.valid_nondep_then h0 parse_common_long (parse_bounded_vlgenbytes 0 token_max_len (parse_bounded_varint 0 token_max_len) `nondep_then` parse_payload_length_pn last pn_length) sl 1ul;
-    LL.valid_nondep_then h0 parse_u32 (parse_bounded_vlbytes 0 20 `nondep_then` parse_bounded_vlbytes 0 20) sl 1ul;
-    let version = LJ.read_u32 sl 1ul in
-    let pos1 = LJ.jump_u32 sl 1ul in
-    LL.valid_nondep_then h0 (parse_bounded_vlbytes 0 20) (parse_bounded_vlbytes 0 20) sl pos1;
-    let dcid = LB.get_vlbytes_contents 0 20 sl pos1 in
-    let dcid_len = LB.bounded_vlbytes_payload_length 0 20 sl pos1 in
-    let pos2 = LB.jump_bounded_vlbytes 0 20 sl pos1 in
-    let scid = LB.get_vlbytes_contents 0 20 sl pos2 in
-    let scid_len = LB.bounded_vlbytes_payload_length 0 20 sl pos2 in
-    let pos3 = LB.jump_bounded_vlbytes 0 20 sl pos2 in
-    LL.valid_nondep_then h0 (parse_bounded_vlgenbytes 0 token_max_len (parse_bounded_varint 0 token_max_len)) (parse_payload_length_pn last pn_length) sl pos3;
-    let token = LB.get_bounded_vlgenbytes_contents 0 token_max_len (read_bounded_varint 0 token_max_len) (jump_bounded_varint 0 token_max_len) sl pos3 in
-    let token_len = LB.bounded_vlgenbytes_payload_length 0 token_max_len (read_bounded_varint 0 token_max_len) sl pos3 in
-    let pos4 = LB.jump_bounded_vlgenbytes 0 token_max_len (jump_bounded_varint 0 token_max_len) (read_bounded_varint 0 token_max_len) sl pos3 in
-    LL.valid_nondep_then h0 parse_varint (parse_packet_number last pn_length) sl pos4;
-    let payload_length = read_varint sl pos4 in
-    let pos5 = jump_varint sl pos4 in
-    let pn = read_packet_number last pn_length sl pos5 in
-//    assert (LL.loc_slice_from_to sl 0ul len `B.loc_includes` B.loc_buffer token);
-    let spec = Impl.BInitial payload_length pn pn_length token token_len in
-    Impl.BLong version dcid dcid_len scid scid_len spec
-
-#pop-options
-
-#push-options "--z3rlimit 128 --z3cliopt smt.arith.nl=false --using_facts_from '*,-FStar.Int.Cast' --query_stats --max_fuel 9 --initial_fuel 9 --max_ifuel 9 --initial_ifuel 9 --query_stats"
-
-#restart-solver
-
-let read_header_body_long_handshake
-  (sl: LL.slice (B.trivial_preorder _) (B.trivial_preorder _))
-  (cid_len: U32.t { U32.v cid_len < 20 } )
-  (last: uint62_t { U64.v last + 1 < pow2 62 })
-  (pn_length: packet_number_length_t)
-: Tot (read_header_body_t sl cid_len last (| Long, (| (), (| Handshake, (| (), (| pn_length, () |) |) |) |) |) )
-= fun len ->
-    let h0 = HST.get () in
-    assert_norm (bitsum'_key_of_t first_byte (| Long, (| (), (| Handshake, (| (), (| pn_length, () |) |) |) |) |) == (| Long, (| (), (| Handshake, (| (), (| pn_length, () |) |) |) |) |) );
-    LL.valid_nondep_then h0 parse_common_long (parse_payload_length_pn last pn_length) sl 1ul;
-    LL.valid_nondep_then h0 parse_u32 (parse_bounded_vlbytes 0 20 `nondep_then` parse_bounded_vlbytes 0 20) sl 1ul;
-    let version = LJ.read_u32 sl 1ul in
-    let pos1 = LJ.jump_u32 sl 1ul in
-    LL.valid_nondep_then h0 (parse_bounded_vlbytes 0 20) (parse_bounded_vlbytes 0 20) sl pos1;
-    let dcid = LB.get_vlbytes_contents 0 20 sl pos1 in
-    let dcid_len = LB.bounded_vlbytes_payload_length 0 20 sl pos1 in
-    let pos2 = LB.jump_bounded_vlbytes 0 20 sl pos1 in
-    let scid = LB.get_vlbytes_contents 0 20 sl pos2 in
-    let scid_len = LB.bounded_vlbytes_payload_length 0 20 sl pos2 in
-    let pos3 = LB.jump_bounded_vlbytes 0 20 sl pos2 in
-    LL.valid_nondep_then h0 parse_varint (parse_packet_number last pn_length) sl pos3;
-    let payload_length = read_varint sl pos3 in
-    let pos4 = jump_varint sl pos3 in
-    let pn = read_packet_number last pn_length sl pos4 in
-    let spec = Impl.BHandshake payload_length pn pn_length in
-    Impl.BLong version dcid dcid_len scid scid_len spec
-
-#restart-solver
-
-let read_header_body_long_ZeroRTT
-  (sl: LL.slice (B.trivial_preorder _) (B.trivial_preorder _))
-  (cid_len: U32.t { U32.v cid_len < 20 } )
-  (last: uint62_t { U64.v last + 1 < pow2 62 })
-  (pn_length: packet_number_length_t)
-: Tot (read_header_body_t sl cid_len last (| Long, (| (), (| ZeroRTT, (| (), (| pn_length, () |) |) |) |) |) )
-= fun len ->
-    let h0 = HST.get () in
-    assert_norm (bitsum'_key_of_t first_byte (| Long, (| (), (| ZeroRTT, (| (), (| pn_length, () |) |) |) |) |) == (| Long, (| (), (| ZeroRTT, (| (), (| pn_length, () |) |) |) |) |) );
-    LL.valid_nondep_then h0 parse_common_long (parse_payload_length_pn last pn_length) sl 1ul;
-    LL.valid_nondep_then h0 parse_u32 (parse_bounded_vlbytes 0 20 `nondep_then` parse_bounded_vlbytes 0 20) sl 1ul;
-    let version = LJ.read_u32 sl 1ul in
-    let pos1 = LJ.jump_u32 sl 1ul in
-    LL.valid_nondep_then h0 (parse_bounded_vlbytes 0 20) (parse_bounded_vlbytes 0 20) sl pos1;
-    let dcid = LB.get_vlbytes_contents 0 20 sl pos1 in
-    let dcid_len = LB.bounded_vlbytes_payload_length 0 20 sl pos1 in
-    let pos2 = LB.jump_bounded_vlbytes 0 20 sl pos1 in
-    let scid = LB.get_vlbytes_contents 0 20 sl pos2 in
-    let scid_len = LB.bounded_vlbytes_payload_length 0 20 sl pos2 in
-    let pos3 = LB.jump_bounded_vlbytes 0 20 sl pos2 in
-    LL.valid_nondep_then h0 parse_varint (parse_packet_number last pn_length) sl pos3;
-    let payload_length = read_varint sl pos3 in
-    let pos4 = jump_varint sl pos3 in
-    let pn = read_packet_number last pn_length sl pos4 in
-    let spec = Impl.BZeroRTT payload_length pn pn_length in
-    Impl.BLong version dcid dcid_len scid scid_len spec
-
-inline_for_extraction
-noextract
-let read_header_body
-  (sl: LL.slice (B.trivial_preorder _) (B.trivial_preorder _))
-  (cid_len: U32.t { U32.v cid_len < 20 } )
-  (last: uint62_t { U64.v last + 1 < pow2 62 })
-  (tg: bitsum'_type first_byte)
-: Tot (read_header_body_t sl cid_len last tg)
-= fun len ->
-  let h0 = HST.get () in
-  match tg with
-  | (| Short, (| (), (spin, (| (), (key_phase, (| pn_length, () |) ) |) ) |) |) ->
-    read_header_body_short sl cid_len last spin key_phase pn_length len
-  | (| Long, (| (), (| Retry, (unused, ()) |) |) |) ->
-    read_header_body_long_retry sl cid_len last unused len
-  | (| Long, (| (), (| Initial, (| (), (| pn_length, () |) |) |) |) |) ->
-    read_header_body_long_initial sl cid_len last pn_length len
-  | (| Long, (| (), (| Handshake, (| (), (| pn_length, () |) |) |) |) |) ->
-    read_header_body_long_handshake sl cid_len last pn_length len
-  | (| Long, (| (), (| ZeroRTT, (| (), (| pn_length, () |) |) |) |) |) ->
-    read_header_body_long_ZeroRTT sl cid_len last pn_length len
-
-#pop-options
-
-#restart-solver
-
-#push-options "--z3rlimit 128 --z3cliopt smt.arith.nl=false --using_facts_from '*,-FStar.Int.Cast' --query_stats"
-
-let read_header
-  packet packet_len cid_len last
-=
-  let h0 = HST.get () in
-  let sl = LL.make_slice packet packet_len in
-  LL.valid_facts (lp_parse_header cid_len last) h0 sl 0ul;
-  assert (B.as_seq h0 packet `Seq.equal` LL.bytes_of_slice_from h0 sl 0ul);
-  let len = validate_header cid_len last sl 0ul in
-  if len `U32.gt` LL.validator_max_length
-  then None
-  else begin
-    let g = Ghost.hide (LL.contents (lp_parse_header cid_len last) h0 sl 0ul) in
-    LL.valid_bitsum_elim
-      #parse_u8_kind
-      #8
-      #U8.t
-      #uint8
-      first_byte
-      #(header' cid_len last)
-      (first_byte_of_header cid_len last)
-      (header_body_type cid_len last)
-      (header_synth cid_len last)
-      parse_u8
-      (parse_header_body cid_len last)
-      h0
-      sl
-      0ul;
-    let r = LJ.read_u8 sl 0ul in
-    let res = destr_first_byte
-      (read_header_body_t sl cid_len last)
-      (fun _ cond dt df len' -> if cond then dt () len' else df () len')
-      (read_header_body sl cid_len last)
-      r
-      len
-    in
-    lemma_header_parsing_post (U32.v cid_len) (U64.v last) (LL.bytes_of_slice_from h0 sl 0ul);
-    Some (res, len)
-  end
-
-let impl_header_length
-  x
-=
-  admit ()
-
-let write_header
-  dst x
-=
-  admit ()
-
-let impl_putative_pn_offset
-  cid_len b len
-=
-  let sl = LowParse.Slice.make_slice b len in
-  let h0 = HST.get () in
-  if not (1ul `U32.lte` cid_len && cid_len `U32.lte` 4ul)
-  then 0ul
-  else
-    let _ = LL.valid_facts parse_u8 h0 sl 0ul in
-    let pos1 = LJ.validate_u8 () sl 0ul in
-    if pos1 `U32.gt` LL.validator_max_length
-    then 0ul
-    else
-      let _ =
-        parser_kind_prop_equiv parse_u8_kind parse_u8;
-        assert (pos1 == 1ul)
-      in
-      let hd = LJ.read_u8 sl 0ul in
-      if uint8.get_bitfield hd 7 8 = 0uy
-      then
-        let _ = LL.valid_facts (parse_bounded_integer (U32.v cid_len)) h0 sl pos1 in
-        let pos2 = LI.validate_bounded_integer' cid_len sl pos1 in
-        if pos2 `U32.gt` LL.validator_max_length
-        then 0ul
-        else pos2
-      else
-        let packet_type = uint8.get_bitfield hd 4 6 in
-        if packet_type = 3uy
-        then 0ul
-        else
-          let _ = LL.valid_facts parse_common_long h0 sl pos1 in
-          let pos2 = validate_common_long sl pos1 in
-          if pos2 `U32.gt` LL.validator_max_length
-          then 0ul
-          else
-            let pos3 =
-              if packet_type = 0uy
-              then
-                let _ = LL.valid_facts (parse_bounded_vlgenbytes 0 token_max_len (parse_bounded_varint 0 token_max_len)) h0 sl pos2 in
-                let pos3 = LB.validate_bounded_vlgenbytes 0 0ul token_max_len (U32.uint_to_t token_max_len) (validate_bounded_varint 0ul (U32.uint_to_t token_max_len)) (read_bounded_varint 0 token_max_len) sl pos2 in
-                if pos3 `U32.gt` LL.validator_max_length
-                then 0ul
-                else pos3
-              else
-                pos2
-            in
-            if pos3 = 0ul
-            then 0ul
-            else
-              let _ = LL.valid_facts parse_varint h0 sl pos3 in
-              let pos4 = validate_varint sl pos3 in
-              if pos4 `U32.gt` LL.validator_max_length
-              then 0ul
-              else pos4
-
-let impl_pn_offset
-  h
-= admit ()
-
-let impl_header_len
-  h
-= admit ()
-
-#pop-options
