src/QUIC.Impl.PacketNumber.fst
@@ -1,0 +1,37 @@
+module QUIC.Impl.PacketNumber
+open QUIC.Spec.Base
+open LowParse.Low.Combinators
+open LowParse.Low.BoundedInt
+
+friend QUIC.Spec.PacketNumber
+
+module Cast = FStar.Int.Cast
+module U64 = FStar.UInt64
+module U32 = FStar.UInt32
+module U16 = FStar.UInt16
+module U8 = FStar.UInt8
+
+let validate_packet_number
+  (last: last_packet_number_t)
+  (pn_len: packet_number_length_t)
+: Tot (validator (parse_packet_number last pn_len))
+= validate_synth
+    (validate_bounded_integer' pn_len)
+    (synth_packet_number last pn_len)
+    ()
+
+let jump_packet_number
+  last pn_len
+= jump_synth
+    (jump_bounded_integer' pn_len)
+    (synth_packet_number last pn_len)
+    ()
+
+let read_packet_number
+  last pn_len
+= read_synth
+    _
+    (synth_packet_number last pn_len)
+    (fun x -> synth_packet_number last pn_len x)
+    (read_bounded_integer' pn_len)
+    ()
