src/QUIC.Impl.PacketNumber.fsti
@@ -1,0 +1,25 @@
+module QUIC.Impl.PacketNumber
+include QUIC.Spec.PacketNumber
+open QUIC.Spec.Base
+open LowParse.Low.Base
+
+module U64 = FStar.UInt64
+module U32 = FStar.UInt32
+
+inline_for_extraction
+val validate_packet_number
+  (last: last_packet_number_t)
+  (pn_len: packet_number_length_t)
+: Tot (validator (parse_packet_number last pn_len))
+
+inline_for_extraction
+val jump_packet_number
+  (last: last_packet_number_t)
+  (pn_len: packet_number_length_t)
+: Tot (jumper (parse_packet_number last pn_len))
+
+inline_for_extraction
+val read_packet_number
+  (last: last_packet_number_t)
+  (pn_len: packet_number_length_t)
+: Tot (leaf_reader (parse_packet_number last pn_len))
