src/QUIC.Spec.PacketNumber.fsti
@@ -1,12 +1,9 @@
-module QUIC.Parse.PacketNumber
+module QUIC.Spec.PacketNumber
 open QUIC.Spec.Base
-open LowParse.Low.Base
+open LowParse.Spec.Base
 
-module Cast = FStar.Int.Cast
 module U64 = FStar.UInt64
 module U32 = FStar.UInt32
-module U16 = FStar.UInt16
-module U8 = FStar.UInt8
 
 inline_for_extraction
 let parse_packet_number_kind
@@ -30,21 +27,3 @@ val serialize_packet_number
   (last: last_packet_number_t)
   (pn_len: packet_number_length_t)
 : Tot (serializer (parse_packet_number last pn_len))
-
-inline_for_extraction
-val validate_packet_number
-  (last: last_packet_number_t)
-  (pn_len: packet_number_length_t)
-: Tot (validator (parse_packet_number last pn_len))
-
-inline_for_extraction
-val jump_packet_number
-  (last: last_packet_number_t)
-  (pn_len: packet_number_length_t)
-: Tot (jumper (parse_packet_number last pn_len))
-
-inline_for_extraction
-val read_packet_number
-  (last: last_packet_number_t)
-  (pn_len: packet_number_length_t)
-: Tot (leaf_reader (parse_packet_number last pn_len))
