src/QUIC.Spec.VarInt.fsti
@@ -1,0 +1,27 @@
+module QUIC.Spec.VarInt
+include QUIC.Spec.Base
+
+module U64 = FStar.UInt64
+module LP = LowParse.Spec.BoundedInt // for bounded_int32
+
+inline_for_extraction
+let parse_varint_kind = {
+  LP.parser_kind_low = 1;
+  LP.parser_kind_high = Some 8;
+  LP.parser_kind_subkind = Some LP.ParserStrong;
+  LP.parser_kind_metadata = None;
+}
+
+val parse_varint : LP.parser parse_varint_kind uint62_t
+
+val serialize_varint : LP.serializer parse_varint
+
+val parse_bounded_varint
+  (min: nat)
+  (max: nat { min <= max /\ max < 4294967296 })
+: Tot (LP.parser parse_varint_kind (LP.bounded_int32 min max))
+
+val serialize_bounded_varint
+  (min: nat)
+  (max: nat { min <= max /\ max < 4294967296 })
+: Tot (LP.serializer (parse_bounded_varint min max))
